proved inv_attestation_consensus_active_instances_predicate_is_in_att_slashing_db_hist

src/dvspec/dafny/att_spec_proofs/incomplete_proofs.dfy
@@ -37,8 +37,38 @@ module Incomplete_Proofs
     ensures inv37(dvn)    
 
 
-    
+    lemma lemma_inv38_inv_attestation_shares_to_broadcast_is_a_subset_of_all_messages_sent(
+        dvn: DVState
+    )
+    requires inv38(dvn)
+    ensures inv_attestation_shares_to_broadcast_is_a_subset_of_all_messages_sent(dvn)
+    {}
 
-    
-    
+    predicate inv_attestation_consensus_active_instances_predicate_is_in_att_slashing_db_hist_body
+    (
+        n_state: DVCNodeState,
+        cid: Slot
+    )
+    {
+        && cid in n_state.attestation_consensus_engine_state.attestation_consensus_active_instances 
+        ==>
+        (
+            && cid in n_state.attestation_consensus_engine_state.att_slashing_db_hist
+            && n_state.attestation_consensus_engine_state.attestation_consensus_active_instances[cid].validityPredicate in n_state.attestation_consensus_engine_state.att_slashing_db_hist[cid] 
+        )
+    }
+
+    predicate inv_attestation_consensus_active_instances_predicate_is_in_att_slashing_db_hist(dvn: DVState)    
+    {
+        forall hn, cid |
+            && hn in dvn.honest_nodes_states.Keys        
+            ::
+            inv_attestation_consensus_active_instances_predicate_is_in_att_slashing_db_hist_body(dvn.honest_nodes_states[hn], cid)
+             
+    }      
+
+    lemma lemma_inv29_inv_attestation_consensus_active_instances_predicate_is_in_att_slashing_db_hist(dvn: DVState)    
+    requires inv29(dvn)
+    ensures inv_attestation_consensus_active_instances_predicate_is_in_att_slashing_db_hist(dvn)
+    {}    
 }
